SEARList.sml
@@ -1,6 +1,4 @@
 
-val lemma = 
- 
 
 
 (*
@@ -44,12 +42,16 @@ fun eq_Pred p  =
 *)
 
 
+(*exists a set of "sets of sets of  pairs (n,a)"
+  (each member of such set is a subset of Pow(N * A), so each such set is  an element of Pow(Pow(N * A)))
+  which satisfies the condition that
+  {} is in the set, and ... *)
 
 val lemma = 
 fVar_Inst 
 [("P",([("sets",mem_sort$ Pow $ Pow $ Cross N (mk_set "A"))],
 “IN(Empty(N * A),sets:mem(Pow(Pow(N * A)))) & 
- !l. IN(l,sets) ==> !a:mem(A).IN(Ins(Pair(Card(l),a),l),sets)”))] 
+ !l. IN(l,sets) ==> !a:mem(A).IN(Ins(Pair(CARD(l),a),l),sets)”))] 
 (IN_def_P_expand |> qspecl [‘Pow(Pow(N * A))’]) 
 
 (*make Ins Pair as Cons0 *)
@@ -60,7 +62,7 @@ val As_def = lemma |> ex2fsym0 "As" ["A"] |> conjE1
 
 
 
-val U_ex_lemma = fVar_Inst 
+val List_ex_lemma = fVar_Inst 
 [("P",([("ls",mem_sort $ Pow $ Cross N (mk_set "A"))],
 “IN(ls,BIGINTER(As(A)))”))]
 (Thm_2_4 |> qspecl [‘(Pow(N * A))’]) 
@@ -71,7 +73,6 @@ $ rewr_fconv (spec_all As_def)
 
 
 
-
 (*f:A->B. is inj, then ?g:B->A. g o f = id(A).
   
 have this function. 
@@ -79,34 +80,694 @@ have this function.
 
 *)
 
-val U_i_def = U_ex_lemma |> ex2fsym0 "U" ["A"] |>ex2fsym0 "i" ["A"]
+val List_LI_def = List_ex_lemma |> ex2fsym0 "List" ["A"] |>ex2fsym0 "LI" ["A"]
+
+val LI_Inj = conjE1 List_LI_def |> gen_all |> store_as "LI_Inj";
+
+val LI_Fun = LI_Inj |> rewr_rule[Inj_def] |> spec_all |> conjE1
+                    |> gen_all |> store_as "LI_Fun";
 
 
-
-val IN_U = U_i_def |> conjE2 |> gen_all |> 
+val IN_List = List_LI_def |> conjE2 |> gen_all |> 
 conv_rule $ basic_once_fconv no_conv (rewr_fconv (eq_sym "mem"))
 |> GSYM
 
 
-val List0 = IN_U  |> allE (rastt "A") |>  allE (rastt "Eval(i(A),b)")
+val List_ind0 = IN_List |> allE (rastt "A") |>  allE (rastt "Eval(LI(A),b)")
                        |> dimp_mp_l2r
-                       (existsI ("b'",mem_sort (rastt "U(A)")) 
-                                (rastt "b:mem(U(A))")
-                                “Eval(i(A), b') = Eval(i(A), b)”
-                                (refl (rastt "Eval(i(A), b)")))
+                       (existsI ("b'",mem_sort (rastt "List(A)")) 
+                                (rastt "b:mem(List(A))")
+                                “Eval(LI(A), b') = Eval(LI(A), b)”
+                                (refl (rastt "Eval(LI(A), b)")))
+                       |> strip_all_and_imp
                        |> gen_all
                        |> disch_all
                        |> gen_all
 
-val List_lemma = prove_store("List_lemma",
+
+val isList_Empty = prove_store("isList_Empty",
+e0
+(strip_tac >> rw[IN_List] >>
+ rpt strip_tac >> arw[])
+(form_goal
+ “!A. ?e. Eval(LI(A),e) = Empty(N * A)”));
+
+val Nil_def = isList_Empty |> spec_all |> ex2fsym0 "Nil" ["A"]
+                           |> gen_all
+                           |> store_as "Nil_def";
+
+val isList_cons = prove_store("isList_cons",
+e0
+(rw[IN_List] >> rpt strip_tac >>
+ first_assum irule >> last_x_assum irule >> arw[])
+(form_goal
+ “!A l. (?l0.Eval(LI(A),l0) = l) ==> !a.?al.Eval(LI(A),al) = Ins(Pair(CARD(l),a),l)”));
+
+(*set of list, takes a list, gives a ser of pairs*)
+
+val sof_ex = prove_store("sof_ex",
+e0
+(rpt strip_tac >> qexists_tac ‘Eval(LI(A),l)’ >> rw[])
+(form_goal
+ “!A l. ?ss. Eval(LI(A),l) = ss”));
+ 
+val sof_def = sof_ex |> spec_all |> ex2fsym0 "sof" ["l"]
+                     |> gen_all |> store_as "sof_def"; 
+
+val Inj_eq = Inj_def |> iffLR |> spec_all |> undisch |> conjE2
+                     |> disch_all |> gen_all
+                     |> store_as "Inj_eq";
+
+local
+val l = 
+fVar_Inst 
+[("P",([("a0l0",mem_sort $ Cross (mk_set "A") (rastt "List(A)")),
+        ("l",mem_sort (rastt "List(A)"))],
+“Ins(Pair(CARD(sof(Snd(a0l0))), Fst(a0l0:mem(A * List(A)))),sof(Snd(a0l0))) = sof(l)”))]
+(AX1 |> qspecl [‘A * List(A)’,‘List(A)’])
+|> uex_expand  
+in
+val Cons_ex = prove_store("Cons_ex",
+e0
+(strip_tac >> strip_assume_tac l >>
+ pop_assum (K all_tac) >> qexists_tac ‘R’ >>
+ arw[Pair_def'] >> rw[Fun_expand] >>
+ arw[] >> rpt strip_tac (* 2 *)
+ >-- (assume_tac isList_cons >>
+     fs[sof_def] >> 
+     pop_assum (qsspecl_then [‘sof(Snd(a))’] assume_tac) >>
+     qby_tac
+     ‘(?l0 : mem(List(A)). sof(l0) = sof(Snd(a)))’ 
+     >-- (qexists_tac ‘Snd(a)’ >> rw[]) >>
+     first_x_assum drule >> 
+     first_x_assum (qspecl_then [‘Fst(a)’] assume_tac) >>
+     pop_assum strip_assume_tac >> qexists_tac ‘al’ >> arw[]) >>
+ irule Inj_eq >> 
+ qexistsl_tac [‘Pow(N * A)’,‘LI(A)’] >> 
+ rw[LI_Inj] >> rw[sof_def] >>
+ pop_assum_list (map_every (assume_tac o GSYM)) >> arw[])
+(form_goal
+ “!A. ?cons:A * List(A) -> List(A).
+  isFun(cons) & 
+  (!a0 l0 l. Holds(cons,Pair(a0,l0),l) <=> 
+  Ins(Pair(CARD(sof(l0)), a0),sof(l0)) = sof(l))”));
+end
+
+val Cons_def = Cons_ex |> spec_all |> ex2fsym0 "Cons" ["A"]
+                       |> gen_all |> store_as "Cons_def";
+
+
+val CONS_ex = prove_store("CONS_ex",
+e0
+(rpt strip_tac >> qexists_tac ‘Eval(Cons(A),Pair(a0,l0))’ >> rw[])
+(form_goal
+ “!A a0 l0. ?l.Eval(Cons(A),Pair(a0,l0)) = l”));
+
+val CONS_def = CONS_ex |> spec_all |> ex2fsym0 "CONS" ["a0","l0"]
+                       |> gen_all |> store_as "CONS_def";
+
+val Eval_Cons = prove_store("Eval_Cons",
+e0
+(rpt strip_tac >>
+ assume_tac Cons_def >> 
+ first_x_assum (qspecl_then [‘A’] strip_assume_tac) >>
+ drule $ GSYM Eval_def >> flip_tac >>
+ arw[] >> lflip_tac >> rw[])
+(form_goal
+ “!A a0 l0 l. Eval(Cons(A), Pair(a0,l0)) = l <=> 
+  Ins(Pair(CARD(sof(l0)),a0),sof(l0)) = sof(l)”));
+
+val Cons_eqn = prove_store("Cons_eqn",
+e0
+(rpt strip_tac >>
+ qsspecl_then [‘a0’,‘l0’,‘Eval(Cons(A), Pair(a0,l0))’] assume_tac
+ Eval_Cons >> fs[])
+(form_goal
+ “!A a0 l0. Ins(Pair(CARD(sof(l0)),a0),sof(l0)) = sof(Eval(Cons(A), Pair(a0,l0)))”));
+
+val CONS_eqn = Cons_eqn |> rewr_rule[CONS_def]
+                        |> store_as "CONS_eqn";
+
+val sof_Nil = Nil_def |> rewr_rule[sof_def] |> store_as "sof_Nil";
+
+val CONS_NOTNIL = prove_store("CONS_NOTNIL",
+e0
+(rpt strip_tac >> ccontra_tac >>
+ qby_tac ‘sof(CONS(a,l)) = sof(Nil(A))’ >-- arw[] >>
+ fs[GSYM CONS_eqn,sof_Nil,Ins_NONEMPTY])
+(form_goal
+ “!A a l. ~(CONS(a,l) = Nil(A))”));
+
+val sof_eq_eq = prove_store("sof_eq_eq",
+e0
+(rpt strip_tac >> dimp_tac >> strip_tac >> arw[] >>
+ fs[GSYM sof_def] >> irule Inj_eq >>
+ qexistsl_tac [‘Pow(N * A)’,‘LI(A)’] >> arw[LI_Inj] )
+(form_goal
+ “!A l1:mem(List(A)) l2.sof(l1) = sof(l2) <=> l1 = l2”));
+
+local
+val l = 
+ fVar_Inst 
+[("P",([("nas",mem_sort$ Pow $ Cross N (mk_set "A"))],
+“?l:mem(List(A)). P(l) & sof(l) = nas”))] 
+(IN_def_P_expand |> qspecl [‘Pow(N * A)’]) 
+in
+val List_ind = prove_store("List_ind",
+e0
+(assume_tac List_ind0 >>
+ rpt strip_tac >>
+ qby_tac
+ ‘?ss. !nas. IN(nas,ss) <=> ?l:mem(List(A)). P(l) & sof(l) = nas’
+ >-- (strip_assume_tac l >> pop_assum (K all_tac) >>
+     qexists_tac ‘s’ >> strip_tac >> pop_assum (assume_tac o GSYM) >>
+     first_x_assum (qspecl_then [‘nas’] accept_tac)) >>
+ pop_assum strip_assume_tac >>
+ qsuff_tac
+ ‘!b. IN(Eval(LI(A),b),ss)’
+ >-- (rpt strip_tac >> 
+     first_x_assum (qspecl_then [‘l’] assume_tac) >>
+     first_x_assum $ drule o iffLR >>
+     pop_assum strip_assume_tac >>
+     pop_assum mp_tac >> once_rw[sof_def] >> once_rw[sof_eq_eq] >>
+     strip_tac >> 
+     assume_tac (EQ_fVar "P" [assume “l' = l:mem(List(A))”]) >>
+     first_x_assum $ irule o iffLR >> 
+     first_x_assum accept_tac) >>
+ (*first_x_assum irule gives err wrong concl*)
+ last_x_assum irule >> rpt strip_tac (* 2 *)
+ >-- (first_assum $ drule o iffLR >> pop_assum strip_assume_tac >>
+     last_assum drule >> 
+     first_assum $ irule o iffRL >>
+     qexists_tac ‘CONS(a',l'')’ >> strip_tac
+     >-- first_assum (qspecl_then [‘a'’] accept_tac) >>
+     qsuff_tac
+     ‘sof(CONS(a', l'')) = Ins(Pair(CARD(sof(l'')), a'), sof(l''))’
+     >-- (qpick_x_assum ‘sof(l'') = l'’ (mp_tac o GSYM) >>
+         pop_assum_list (map_every (K all_tac)) >> rpt strip_tac >>
+         arw[]) >>
+     once_rw[CONS_eqn]  >> rw[]) >>
+ first_assum $ irule o iffRL >>
+ qexists_tac ‘Nil(A)’ >> strip_tac 
+ >-- first_assum accept_tac >>
+ once_rw[GSYM Nil_def] >> rw[sof_def]
+ )
+(form_goal
+ “!A. P(Nil(A)) & 
+      (!l:mem(List(A)). P(l) ==> !a. P(CONS(a,l))) ==>
+     !l:mem(List(A)).P(l) ”));
+end
+
+
+
+
+local 
+val l = 
+ fVar_Inst 
+[("P",([("l",mem_sort (rastt "List(A)"))],
+“Fin(sof(l:mem(List(A))))”))] 
+(List_ind |> qspecl [‘A’]) 
+in
+val LI_Fin = prove_store("LI_Fin",
+e0
+(strip_tac >> match_mp_tac l >>
+ rw[sof_Nil,Fin_Empty] >> rpt strip_tac >>
+ rw[GSYM CONS_eqn] >> drule Fin_Ins >> arw[])
+(form_goal
+ “!A l:mem(List(A)). Fin(sof(l))”));
+end
+
+
+local
+val l = 
+ fVar_Inst 
+[("P",([("l",mem_sort (rastt "List(A)"))],
+“!n a:mem(A). IN(Pair(n,a),sof(l)) ==> Lt(n,CARD(sof(l)))”))] 
+(List_ind |> qspecl [‘A’])
+in
+val isList_CARD_NOTIN0 = prove_store("isList_CARD_NOTIN0",
+e0
+(strip_tac >> strip_tac >> strip_tac >> strip_tac >> match_mp_tac l >>
+ rpt strip_tac (* 2 *)
+ >-- fs[sof_Nil,Empty_property] >>
+ fs[GSYM CONS_eqn,IN_Ins] (* 2 *)
+ >-- (fs[Pair_eq_eq] >> 
+     qby_tac ‘~IN(Pair(CARD(sof(l')), a'),sof(l'))’ 
+     >-- (ccontra_tac >> first_x_assum drule  >>
+         fs[Lt_def]) >>
+     qsspecl_then [‘l'’] assume_tac LI_Fin >>
+     drule CARD_Ins >> first_x_assum drule >> 
+     arw[] >> rw[Lt_Suc]) >>
+ first_x_assum drule >> 
+ cases_on “IN(Pair(CARD(sof(l')), a':mem(A)),sof(l'))” 
+ >-- (drule Ins_absorb >> arw[]) >>
+ qsspecl_then [‘l'’] assume_tac LI_Fin >>
+ drule CARD_Ins >> first_x_assum drule >> arw[] >>
+ irule Lt_trans >>
+ qexists_tac ‘CARD(sof(l'))’ >> arw[Lt_Suc])
+(form_goal
+ “!A l n a:mem(A). IN(Pair(n,a),sof(l)) ==> Lt(n,CARD(sof(l)))”));
+end
+
+
+val Cons_Inj = prove_store("Cons_Inj",
+e0
+(strip_tac >> rw[Inj_def,Cons_def] >> 
+ rpt strip_tac >>
+ qsspecl_then [‘x1’]
+ (x_choosel_then ["a1","l1"] assume_tac) Pair_has_comp >>
+ qsspecl_then [‘x2’] 
+ (x_choosel_then ["a2","l2"] assume_tac) Pair_has_comp >>
+ fs[] >> fs[CONS_def] >> 
+ qby_tac
+ ‘sof(CONS(a1, l1)) = sof(CONS(a2, l2))’
+ >-- arw[] >>
+ fs[GSYM CONS_eqn] >>
+ qsuff_tac
+ ‘Pair(CARD(sof(l1)), a1) = Pair(CARD(sof(l2)), a2) & 
+  sof(l1) = sof(l2)’
+ >-- (rw[Pair_eq_eq,sof_eq_eq] >> rpt strip_tac >> arw[]) >>
+ irule Ins_eq_eq >>
+ arw[] >>
+ qby_tac
+ ‘~IN(Pair(CARD(sof(l1)), a1), sof(l1))’
+ >-- (ccontra_tac >> drule isList_CARD_NOTIN0 >> fs[Lt_def]) >>
+ qby_tac
+ ‘~IN(Pair(CARD(sof(l2)), a2), sof(l2))’
+ >-- (ccontra_tac >> drule isList_CARD_NOTIN0 >> fs[Lt_def]) >>
+ arw[] >>
+ qby_tac ‘CARD(sof(l2)) = CARD(sof(l1))’ 
+ >-- (drule $ GSYM Del_Ins >> rev_drule $ GSYM Del_Ins >>  
+     once_arw[] >> pop_assum (K all_tac) >>
+     pop_assum (K all_tac) >>
+     qsspecl_then [‘l2’] assume_tac LI_Fin >>
+     drule CARD_Ins >>
+     first_x_assum drule >> 
+     drule Fin_Ins >>
+     first_x_assum (qspecl_then [‘Pair(CARD(sof(l2)), a2)’] assume_tac)>>
+     drule CARD_Del >>
+     first_x_assum (qspecl_then [‘Pair(CARD(sof(l2)), a2)’] assume_tac) >>
+     pop_assum mp_tac >> rw[IN_Ins] >>
+     strip_tac >> 
+     qsuff_tac
+     ‘Pre(CARD(Ins(Pair(CARD(sof(l2)), a2), sof(l2)))) = 
+      CARD(Del(Ins(Pair(CARD(sof(l1)), a1), sof(l1)),
+                 Pair(CARD(sof(l1)), a1)))’
+     >-- (strip_tac >> arw[]) >>
+     pop_assum (K all_tac) >> pop_assum (K all_tac) >>
+     pop_assum (K all_tac) >> pop_assum (K all_tac) >>
+     qsspecl_then [‘l1’] assume_tac LI_Fin >>
+     drule CARD_Ins >> 
+     first_x_assum drule >>
+     drule Fin_Ins >>
+     first_x_assum (qspecl_then [‘Pair(CARD(sof(l1)), a1)’] assume_tac)>>
+     drule CARD_Del >>
+     first_x_assum (qspecl_then [‘Pair(CARD(sof(l1)), a1)’] assume_tac) >>
+     pop_assum mp_tac >> rw[IN_Ins] >>
+     strip_tac >> once_arw[] >>
+     qpick_x_assum
+     ‘Ins(Pair(CARD(sof(l1)), a1), sof(l1)) =
+               Ins(Pair(CARD(sof(l2)), a2), sof(l2))’ mp_tac >>
+     pop_assum_list (map_every (K all_tac)) >>
+     strip_tac >> arw[]) >>
+ strip_tac (* 2 *)
+ >-- (pop_assum (assume_tac o GSYM) >> arw[] >>
+     ccontra_tac >> drule isList_CARD_NOTIN0 >> fs[Lt_def]) >>
+ arw[] >> ccontra_tac >> drule isList_CARD_NOTIN0 >> fs[Lt_def]
+ )
+(form_goal
+ “!A. isInj(Cons(A))”));
+
+
+val CONS_eq_eq = prove_store("CONS_eq_eq",
+e0
+(rw[GSYM CONS_def] >> rpt strip_tac >> dimp_tac >> strip_tac >> arw[] >>
+ irule $ iffLR Pair_eq_eq >>
+ irule Inj_eq >>
+ qexistsl_tac [‘List(A)’,‘Cons(A)’] >> arw[Cons_Inj])
+(form_goal
+ “!A a1:mem(A) l1 a2 l2.CONS(a1,l1) = CONS(a2,l2) <=> (a1 = a2 & l1 = l2)”));
+
+
+
+
+local
+val l = 
+ fVar_Inst 
+[("P",([("l",mem_sort (rastt "List(A)"))],
+“l = Nil(A) | ?a0 l0. l = CONS(a0, l0)”))] 
+(List_ind |> qspecl [‘A’])
+in
+val CONS_or_Nil = prove_store("CONS_or_Nil",
+e0
+(strip_tac >> irule l >> rw[] >>
+ rpt strip_tac >--
+ (rw[CONS_NOTNIL] >> qexistsl_tac [‘a’,‘l'’] >> rw[]) >>
+ rw[CONS_NOTNIL] >> 
+ qexistsl_tac [‘a’,‘l'’] >> arw[])
+(form_goal
+ “!A l:mem(List(A)). l = Nil(A) | ?a0 l0. l = CONS(a0,l0)”));
+end
+
+local
+val l = 
+ fVar_Inst 
+[("P",([("l",mem_sort (rastt "List(A)"))],
+“Eval(f1:List(A) ->X, l) = Eval(f2, l)”))] 
+(List_ind |> qspecl [‘A’])
+in
+val from_List_eq = prove_store("from_List_eq",
+e0
+(rpt strip_tac >> irule $ iffRL FUN_EXT >> arw[] >>
+ irule l >> arw[])
+(form_goal
+ “!A X f1:List(A) ->X f2. isFun(f1) & isFun(f2) &
+ Eval(f1, Nil(A)) = Eval(f2,Nil(A)) &
+ (!l. Eval(f1,l) = Eval(f2,l) ==> 
+  !a. Eval(f1,CONS(a,l)) = Eval(f2,CONS(a,l))) ==> f1 = f2”));
+end
+
+
+
+val cRf_def = 
+fVar_Inst 
+[("P",([("ss",mem_sort$ Pow $ Cross (rastt "List(A)") (mk_set "X"))],
+“IN(Pair(Nil(A),x:mem(X)),ss)& 
+ !l x. IN(Pair(l,x),ss) ==> 
+    !a:mem(A).IN(Pair(CONS(a,l),Eval(t,Pair(a,x))),ss)”))] 
+(IN_def_P_expand |> qspecl [‘Pow(List(A) * X)’]) 
+|> ex2fsym0 "cRf" ["x","t"] |> conjE1 
+|> qgen ‘t’ |> qgen ‘A’
+|> gen_all |> GSYM
+
+local
+val Rf0_ex = 
+fVar_Inst 
+[("P",([("lx",mem_sort $ Cross (rastt "List(A)") (mk_set "X"))],
+“IN(lx,BIGINTER(cRf(x:mem(X),t:A * X->X)))”))]
+(Thm_2_4 |> qspecl [‘List(A) * X’]) 
+|> conv_rule $ once_depth_fconv no_conv 
+$ rewr_fconv (spec_all IN_BIGINTER)
+|> conv_rule $ once_depth_fconv no_conv 
+$ rewr_fconv (spec_all cRf_def) |> GSYM
+val R = 
+fVar_Inst 
+[("P",([("l",mem_sort (rastt "List(A)")),("x",mem_sort (mk_set "X"))],
+“?r.Eval(i:B-> List(A) * X,r) = Pair(l,x)”))]
+(AX1 |> qspecl [‘List(A)’,‘X’]) |> uex_expand
+val ss = fVar_Inst 
+[("P",([("lx",mem_sort $ Cross (rastt "List(A)") (mk_set "X"))],
+“Holds(P:List(A) ->X,Fst(lx),Snd(lx))”))] 
+(IN_def_P_expand |> qspecl [‘List(A) * X’]) 
+in
+val Rf_ex = prove_store("Rf_ex",
+e0
+(rpt strip_tac >> strip_assume_tac Rf0_ex >>
+ strip_assume_tac R >>
+ pop_assum (K all_tac) >>
+ qexists_tac ‘R’ >>
+ strip_tac (* 2 *)
+ >-- (arw[] >> flip_tac >> arw[] >>
+     rpt strip_tac >> arw[]) >> strip_tac (* 2 *)
+ >-- (arw[] >> flip_tac >> arw[] >> rpt strip_tac >>
+     first_assum irule >> first_assum irule >> arw[]) >>
+ arw[] >> flip_tac >>
+ arw[] >> rpt strip_tac >>
+ strip_assume_tac ss >> pop_assum (K all_tac) >>
+ first_x_assum (qspecl_then [‘s’] assume_tac) >>
+ first_assum (qspecl_then [‘Pair(l,x0)’] assume_tac) >>
+ fs[Pair_def'] >>
+ first_assum irule >> strip_tac (* 2 *)
+ >-- (strip_tac >> strip_tac >> 
+     first_assum (qspecl_then [‘Pair(l',x')’] (assume_tac o GSYM)) >> 
+     once_arw[] >> rw[Pair_def'] >> 
+     rpt strip_tac >> first_x_assum drule >>
+     qpick_x_assum
+     ‘!a. Holds(P, Fst(a), Snd(a)) <=> IN(a, s)’ (assume_tac o GSYM) >>
+     once_arw[] >> rw[Pair_def'] >> once_arw[]) >>
+ qpick_x_assum
+     ‘!a. Holds(P, Fst(a), Snd(a)) <=> IN(a, s)’ (assume_tac o GSYM) >> 
+  once_arw[] >> rw[Pair_def'] >> 
+ first_x_assum accept_tac
+ )
+(form_goal
+ “!X x A t:A * X ->X. ?Rf:List(A) ->X.
+ Holds(Rf,Nil(A),x) & 
+ (!l x0. Holds(Rf,l,x0) ==> !a. Holds(Rf,CONS(a,l),Eval(t,Pair(a,x0)))) &
+ (!P.
+ (Holds(P,Nil(A),x) & 
+  (!l x0. Holds(P,l,x0) ==> !a. Holds(P,CONS(a,l),Eval(t,Pair(a,x0)))))
+  ==> !l x0.Holds(Rf,l,x0) ==> Holds(P,l,x0))”));
+end
+
+val Rf_def = Rf_ex |> spec_all
+                   |> ex2fsym0 "Rf" ["x","t"]
+                   |> qgen ‘t’ |> qgen ‘A’
+                   |> gen_all |> store_as "Rf_def";
+
+val Rf_property = conjI (Rf_def |> spec_all |> conjE1)
+                        (Rf_def |> spec_all |> conjE2 |> conjE1)
+                        |> qgen ‘t’ |> qgen ‘A’
+                        |> gen_all |> store_as "Rf_property";
+
+val Rf_min = Rf_def |> spec_all |> conjE2 |> conjE2
+                    |> qgen ‘t’ |> qgen ‘A’
+                    |> gen_all |> store_as "Rf_property";
+
+local
+val P = 
+fVar_Inst 
+[("P",([("l1",mem_sort (rastt "List(A)")),("x1",mem_sort (mk_set "X"))],
+“Holds(Rf(x,t:A * X->X),l1,x1) & ~(l1 = Nil(A) & x1 = x0)”))]
+(AX1 |> qspecl [‘List(A)’,‘X’]) |> uex_expand
+in
+val Rf_Nil_unique = prove_store("Rf_Nil_unique",
+e0
+(rpt strip_tac >> ccontra_tac >>
+ qsuff_tac
+ ‘?P. Holds(P,Nil(A),x) & 
+     (!l x0. Holds(P,l,x0) ==>
+      !a. Holds(P,CONS(a,l),Eval(t,Pair(a,x0)))) & 
+     ~Holds(P,Nil(A),x0)’ 
+ >-- (strip_tac >> qsspecl_then [‘x’,‘t’,‘P’] assume_tac Rf_min >>
+     qsuff_tac ‘Holds(P, Nil(A), x0)’ >--arw[] >>
+     first_x_assum irule >> arw[Rf_property]) >>
+ qsuff_tac
+ ‘?P. !l1 x1. Holds(P,l1,x1) <=> 
+  Holds(Rf(x,t),l1,x1) & ~(l1 = Nil(A) & x1 = x0)’
+ >-- (strip_tac >> qexists_tac ‘P’ >> arw[] >>
+     rw[Rf_property] >> flip_tac >> arw[] >>
+     (*do not understand why need strip*)
+     strip_tac >> strip_tac >> arw[] >> 
+     rw[CONS_NOTNIL] >> rpt strip_tac >>  
+     qsspecl_then [‘x’,‘t’] strip_assume_tac Rf_property >>
+      last_x_assum (K all_tac) >>
+      first_x_assum rev_drule >> arw[]) >>
+ strip_assume_tac P >> 
+ qexists_tac ‘R’ >> arw[]
+ )
+(form_goal
+ “!X x A t:A * X ->X x0. 
+  Holds(Rf(x,t),Nil(A),x0) ==> x0 = x”));
+end
+
+val Rf_CONS = Rf_property |> spec_all |> conjE2
+                          |> qgen ‘t’ |> qgen ‘A’
+                          |> gen_all
+                          |> store_as "Rf_CONS";
+
+
+local
+val P = 
+fVar_Inst 
+[("P",([("l0",mem_sort (rastt "List(A)")),("x0",mem_sort (mk_set "X"))],
+“Holds(Rf(x,t:A * X ->X),l0,x0) & 
+  !a l1. l0 = CONS(a,l1) ==> 
+  ?x1. Holds(Rf(x,t),l1,x1) & x0 = Eval(t,Pair(a,x1))”))]
+(AX1 |> qspecl [‘List(A)’,‘X’]) |> uex_expand
+in
+val Rf_Cons_back = prove_store("Rf_Cons_back",
+e0
+(strip_tac >> strip_tac >> strip_tac >> strip_tac >> 
+ qby_tac
+ ‘?P. !l0 x0. Holds(P,l0,x0) <=>
+  Holds(Rf(x,t),l0,x0) & 
+  !a l1. l0 = CONS(a,l1) ==> 
+  ?x1. Holds(Rf(x,t),l1,x1) & x0 = Eval(t,Pair(a,x1))’ 
+ >-- (strip_assume_tac P >> qexists_tac ‘R’ >> arw[]) >>
+ pop_assum strip_assume_tac >>
+  qsuff_tac
+ ‘!l0 x0.Holds(Rf(x, t),l0, x0) ==> Holds(P,l0,x0)’
+ >-- arw[] >>
+ match_mp_tac Rf_min >>
+ arw[] >> rw[GSYM CONS_NOTNIL] >> rpt strip_tac (* 3 *)
+ >-- rw[Rf_property]
+ >-- (drule Rf_CONS >> arw[]) >>
+ qsspecl_then [‘l’] strip_assume_tac CONS_or_Nil >-- (* 2 *)
+ (fs[CONS_eq_eq] >> qexists_tac ‘x0'’ >> arw[]) >>
+ fs[CONS_eq_eq] >> qexists_tac ‘x0'’ >> arw[]
+)
+(form_goal
+ “!X x A t:A * X ->X l0 x0. Holds(Rf(x,t),l0,x0) ==>
+  Holds(Rf(x,t),l0,x0) & 
+  !a l1. l0 = CONS(a,l1) ==> 
+  ?x1. Holds(Rf(x,t),l1,x1) & x0 = Eval(t,Pair(a,x1))”));
+end
+
+
+
+
+local
+val P = 
+fVar_Inst 
+[("P",([("l0",mem_sort (rastt "List(A)")),("x0",mem_sort (mk_set "X"))],
+“(!x'. Holds(Rf(x,t:A * X ->X),l0,x')  ==> x' = x0)”))]
+(AX1 |> qspecl [‘List(A)’,‘X’]) |> uex_expand
+in
+val Rf_unique = prove_store("Rf_unique",
+e0
+(strip_tac >> strip_tac >> strip_tac >> strip_tac >> 
+ qby_tac
+ ‘?P. !l0 x0. Holds(P,l0,x0) <=>
+ (!x'. Holds(Rf(x,t),l0,x')  ==> x' = x0)’
+ >-- (strip_assume_tac P >> qexists_tac ‘R’ >> arw[]) >> 
+ pop_assum strip_assume_tac >>
+ qsuff_tac 
+ ‘!l0 x0. Holds(Rf(x,t),l0,x0) ==> Holds(P,l0,x0)’ 
+ >-- arw[] >>
+ match_mp_tac Rf_min >> arw[] >> 
+ strip_tac (* 2 *)
+ >-- rw[Rf_Nil_unique] >> rpt strip_tac >>
+ drule Rf_Cons_back >> 
+ pop_assum strip_assume_tac >>
+ first_x_assum (qspecl_then [‘a’,‘l’] assume_tac) >> fs[] >>
+ first_x_assum drule >> arw[])
+(form_goal
+ “!X x A t:A * X ->X l0 x0. 
+  Holds(Rf(x,t),l0,x0) ==>
+  !x'. Holds(Rf(x,t),l0,x') ==> x' = x0”));
+end
+
+local 
+val l = 
+ fVar_Inst 
+[("P",([("l0",mem_sort (rastt "List(A)"))],
+“?!x0. Holds(Rf(x, t:A * X ->X), l0, x0)”))] 
+(List_ind |> qspecl [‘A’]) 
+in
+val Rf_uex = prove_store("Rf_uex",
+e0
+(rpt strip_tac >>
+ irule l >> rpt strip_tac (* 2 *)
+ >-- (pop_assum (strip_assume_tac o uex_expand) >>
+     drule Rf_CONS >>
+ first_x_assum (qspecl_then [‘a’] assume_tac) >>
+ uex_tac >> qexists_tac ‘Eval(t, Pair(a,x0))’ >> arw[] >> drule Rf_unique >> arw[]) >>
+ uex_tac >> qexists_tac ‘x’ >> rw[Rf_property] >>
+ rw[Rf_Nil_unique])
+(form_goal
+ “!X x A t:A * X ->X l0.?!x0. Holds(Rf(x,t),l0,x0)”));
+end
+
+
+
+val List_rec = prove_store("List_rec",
+e0
+(rpt strip_tac >> uex_tac >> 
+ assume_tac Rf_uex >> qexists_tac ‘Rf(x,t)’ >>
+ qby_tac
+ ‘isFun(Rf(x,t))’
+ >-- arw[Fun_def] >>
+ arw[] >> 
+ qby_tac
+ ‘Eval(Rf(x, t), Nil(A)) = x &
+               Rf(x, t) o Cons(A) = t o
+                 Pa(p1(A, List(A)), Rf(x, t) o p2(A, List(A)))’
+ >-- (drule $GSYM Eval_def >> flip_tac >> arw[Rf_property] >>
+     irule $ iffRL FUN_EXT >>
+     qby_tac ‘isFun(Rf(x, t) o Cons(A))’
+     >-- (irule o_Fun >> arw[Cons_def]) >> arw[] >>
+     qby_tac ‘isFun(t o Pa(p1(A, List(A)), Rf(x, t) o p2(A, List(A))))’
+     >-- (irule o_Fun >> arw[] >> irule Pa_Fun >>
+         rw[p1_Fun] >> irule o_Fun >> arw[p2_Fun]) >>
+     arw[] >> strip_tac >>
+     assume_tac Rf_CONS >>
+     qsspecl_then [‘a’] (x_choosel_then ["l","x0"] assume_tac)
+     Pair_has_comp >> fs[] >>
+     irule $ iffRL Eval_o_l >> rw[CONS_def] >>
+     arw[Cons_def] >> flip_tac >>
+     irule $ iffRL Eval_o_l >>
+     arw[] >> rpt strip_tac  (* 2 *)
+     >-- (qby_tac
+         ‘isFun(p1(A, List(A))) & 
+          isFun(Rf(x, t) o p2(A, List(A)))’
+         >-- (rw[p1_Fun] >> irule o_Fun >> arw[p2_Fun]) >>
+         drule Eval_Pa_Pair >> arw[] >> rw[Eval_p1_Pair] >>
+         qby_tac ‘isFun(p2(A, List(A))) & isFun(Rf(x,t))’
+         >-- arw[p2_Fun] >>
+         drule$ GSYM o_Eval' >> arw[] >> rw[Eval_p2_Pair] >>
+         first_x_assum irule >> 
+         irule Holds_Eval >> arw[]) >>
+     irule Pa_Fun >> rw[p1_Fun] >> irule o_Fun >>
+     arw[p2_Fun]) >>
+ arw[] >> rpt strip_tac >>
+ irule from_List_eq >>
+ arw[] >> rpt strip_tac >>
+ rw[GSYM CONS_def] >>
+ irule $ iffLR Eval_o_l >> arw[] >> 
+ rw[Cons_def] >>
+ irule $ iffRL Eval_o_l >> arw[] >> 
+ qby_tac
+ ‘isFun(p1(A, List(A))) & isFun(f' o p2(A, List(A)))’
+ >-- (rw[p1_Fun] >> irule o_Fun >> arw[p2_Fun]) >>
+ drule Eval_Pa_Pair >> arw[] >> rw[Eval_p1_Pair] >>
+ qby_tac ‘isFun(p2(A,List(A))) & isFun(f')’ 
+ >-- arw[p2_Fun] >>
+ drule $GSYM o_Eval' >> arw[] >> rw[Eval_p2_Pair] >>
+ arw[] >> strip_tac (* 2 *)
+ >-- (flip_tac >> irule $ iffLR Eval_o_l >> arw[Cons_def] >>
+     irule $ iffRL Eval_o_l >> arw[] >>
+     strip_tac (* 2 *)
+     >-- (irule Eval_input_eq >> 
+         qby_tac ‘isFun(p1(A, List(A))) & isFun(Rf(x,t) o p2(A, List(A)))’
+         >-- (rw[p1_Fun] >> irule o_Fun >> arw[p2_Fun]) >>
+         drule Eval_Pa_Pair >> arw[] >>
+         rw[Eval_p1_Pair] >> rw[Pair_eq_eq] >>
+         irule $ iffRL Eval_o_l >> arw[p2_Fun,Eval_p2_Pair]) >>
+     irule Pa_Fun >> rw[p1_Fun] >> irule o_Fun >>
+     arw[p2_Fun]) >>
+ irule Pa_Fun >> rw[p1_Fun] >> irule o_Fun >>
+ arw[p2_Fun])
+(form_goal
+ “!X x A t:A * X ->X. isFun(t) ==> 
+  ?!f:List(A) -> X. isFun(f) & Eval(f,Nil(A)) = x &
+      f o Cons(A) = t o Pa(p1(A,List(A)), f o p2(A,List(A)))”));
+
+
+(*
+val Rf_ex = prove_store("Rf_ex",
 e0
 ()
 (form_goal
- “!A b. ”));
+ “!X x:1->X A t:A * X ->X 
+  ?Rf. 
+
+!l0 x0.Holds(Rf,l0,x0) = TRUE ==>
+  Rf(x,t) o Pa(l0,x0) = TRUE & 
+  !a l1. l0 = CONS(a,l1) ==> 
+  ?x1. Rf(x,t) o Pa(l1,x1) = TRUE & x0 = t o Pa(a,x1)”));
+
+val Rf_def  = 
+
+*)
+
+val isList_property = prove_store("isList_property",
+e0
+()
+(form_goal “!A l:List(A). 
+ !
+ ”));
 
 
-val _ = new_pred "hasCard" [("xs",mem_sort $Pow (mk_set "X")),("n",mem_sort N)]
-val hasCard_def = store_ax("hasCard_def",
-“!X xs:mem(Pow(X)) n.hasCard(xs,n) <=> Holds(Card(X),xs,n)”)
 
-val Card_def' = Card_lemma |> rewr_rule[GSYM hasCard_def]
+
